Refactoring substitution parameter order

matching-logic/src/PatternContext.v
@@ -17,6 +17,8 @@ Require Import
     Substitution
 .
 
+Import MatchingLogic.Substitution.Notations.
+
 Section with_signature.
     Context {Σ : Signature}.
 
@@ -29,8 +31,9 @@ Section with_signature.
 
   Definition PC_wf C := well_formed (pcPattern C).
 
+  Open Scope ml_scope.
   Definition emplace (ctx : PatternCtx) (p : Pattern) : Pattern :=
-    free_evar_subst (pcPattern ctx) p (pcEvar ctx).
+    (pcPattern ctx)^[[evar: (pcEvar ctx) ↦ p]].
 
 
 End with_signature.
