matching-logic/src/Substitution.v
@@ -15,7 +15,7 @@ Section subst.
 
      (* There are two substitution operations over patterns, [bevar_subst] and [bsvar_subst]. *)
   (* substitute bound variable x for psi in phi *)
-  Fixpoint bevar_subst (phi psi : Pattern) (x : db_index) :=
+  Fixpoint bevar_subst (x : db_index) (psi phi : Pattern) :=
     match phi with
     | patt_free_evar x' => patt_free_evar x'
     | patt_free_svar x' => patt_free_svar x'
@@ -26,15 +26,15 @@ Section subst.
                            end
     | patt_bound_svar n => patt_bound_svar n
     | patt_sym sigma => patt_sym sigma
-    | patt_app phi1 phi2 => patt_app (bevar_subst phi1 psi x)
-                                     (bevar_subst phi2 psi x)
+    | patt_app phi1 phi2 => patt_app (bevar_subst x psi phi1)
+                                     (bevar_subst x psi phi2)
     | patt_bott => patt_bott
-    | patt_imp phi1 phi2 => patt_imp (bevar_subst phi1 psi x) (bevar_subst phi2 psi x)
-    | patt_exists phi' => patt_exists (bevar_subst phi' psi (S x))
-    | patt_mu phi' => patt_mu (bevar_subst phi' psi x)
+    | patt_imp phi1 phi2 => patt_imp (bevar_subst x psi phi1) (bevar_subst x psi phi2)
+    | patt_exists phi' => patt_exists (bevar_subst (S x) psi phi')
+    | patt_mu phi' => patt_mu (bevar_subst x psi phi')
     end.
 
-  Fixpoint bsvar_subst (phi psi : Pattern) (x : db_index) :=
+  Fixpoint bsvar_subst (x : db_index) (psi phi : Pattern) :=
     match phi with
     | patt_free_evar x' => patt_free_evar x'
     | patt_free_svar x' => patt_free_svar x'
@@ -45,12 +45,12 @@ Section subst.
                            | Nat_greater _ _ _ => patt_bound_svar (Nat.pred n)
                            end
     | patt_sym sigma => patt_sym sigma
-    | patt_app phi1 phi2 => patt_app (bsvar_subst phi1 psi x)
-                                     (bsvar_subst phi2 psi x)
+    | patt_app phi1 phi2 => patt_app (bsvar_subst x psi phi1)
+                                     (bsvar_subst x psi phi2)
     | patt_bott => patt_bott
-    | patt_imp phi1 phi2 => patt_imp (bsvar_subst phi1 psi x) (bsvar_subst phi2 psi x)
-    | patt_exists phi' => patt_exists (bsvar_subst phi' psi x)
-    | patt_mu phi' => patt_mu (bsvar_subst phi' psi (S x))
+    | patt_imp phi1 phi2 => patt_imp (bsvar_subst x psi phi1) (bsvar_subst x psi phi2)
+    | patt_exists phi' => patt_exists (bsvar_subst x psi phi')
+    | patt_mu phi' => patt_mu (bsvar_subst (S x) psi phi')
     end.
 
 
@@ -85,44 +85,65 @@ Section subst.
     end.
   
   (* substitute free element variable x for psi in phi *)
-  Fixpoint free_evar_subst (phi psi : Pattern) (x : evar) :=
+  Fixpoint free_evar_subst (x : evar) (psi phi : Pattern) :=
     match phi with
     | patt_free_evar x' => if decide (x = x') is left _ then psi else patt_free_evar x'
     | patt_free_svar X => patt_free_svar X
     | patt_bound_evar x' => patt_bound_evar x'
     | patt_bound_svar X => patt_bound_svar X
     | patt_sym sigma => patt_sym sigma
-    | patt_app phi1 phi2 => patt_app (free_evar_subst phi1 psi x)
-                                     (free_evar_subst phi2 psi x)
+    | patt_app phi1 phi2 => patt_app (free_evar_subst x psi phi1)
+                                     (free_evar_subst x psi phi2)
     | patt_bott => patt_bott
-    | patt_imp phi1 phi2 => patt_imp (free_evar_subst phi1 psi x) (free_evar_subst phi2 psi x)
-    | patt_exists phi' => patt_exists (free_evar_subst phi' psi x)
-    | patt_mu phi' => patt_mu (free_evar_subst phi' psi x)
+    | patt_imp phi1 phi2 => patt_imp (free_evar_subst x psi phi1) (free_evar_subst x psi phi2)
+    | patt_exists phi' => patt_exists (free_evar_subst x psi phi')
+    | patt_mu phi' => patt_mu (free_evar_subst x psi phi')
     end.
 
   (* substitute free set variable X for psi in phi *)
-  Fixpoint free_svar_subst (phi psi : Pattern) (X : svar) : Pattern :=
+  Fixpoint free_svar_subst (X : svar) (psi phi : Pattern) : Pattern :=
     match phi with
     | patt_free_evar x => patt_free_evar x
     | patt_free_svar X' => if decide (X = X') is left _ then psi else patt_free_svar X'
     | patt_bound_evar x => patt_bound_evar x
     | patt_bound_svar X' => patt_bound_svar X'
     | patt_sym sigma => patt_sym sigma
-    | patt_app phi1 phi2 => patt_app (free_svar_subst phi1 psi X)
-                                     (free_svar_subst phi2 psi X)
+    | patt_app phi1 phi2 => patt_app (free_svar_subst X psi phi1)
+                                     (free_svar_subst X psi phi2)
     | patt_bott => patt_bott
-    | patt_imp phi1 phi2 => patt_imp (free_svar_subst phi1 psi X) (free_svar_subst phi2 psi X)
-    | patt_exists phi' => patt_exists (free_svar_subst phi' psi X)
-    | patt_mu phi' => patt_mu (free_svar_subst phi' psi X)
+    | patt_imp phi1 phi2 => patt_imp (free_svar_subst X psi phi1) (free_svar_subst X psi phi2)
+    | patt_exists phi' => patt_exists (free_svar_subst X psi phi')
+    | patt_mu phi' => patt_mu (free_svar_subst X psi phi')
     end.
+
 
   (* instantiate exists x. p or mu x. p with psi for p *)
   Definition instantiate (phi psi : Pattern) :=
     match phi with
-    | patt_exists phi' => bevar_subst phi' psi 0
-    | patt_mu phi' => bsvar_subst phi' psi 0
+    | patt_exists phi' => bevar_subst 0 psi phi'
+    | patt_mu phi' => bsvar_subst 0 psi phi'
     | _ => phi
     end.
+End subst.
+
+Module Notations.
+
+  Declare Scope ml_scope.
+  Notation "e ^[ 'evar:' dbi ↦ e' ]" := (bevar_subst dbi e' e) (at level 2, e' at level 200, left associativity,
+  format "e ^[ 'evar:' dbi ↦ e' ]" ) : ml_scope.
+  Notation "e ^[ 'svar:' dbi ↦ e' ]" := (bsvar_subst dbi e' e) (at level 2, e' at level 200, left associativity,
+  format "e ^[ 'svar:' dbi ↦ e' ]" ) : ml_scope.
+  Notation "e ^[[ 'evar:' x ↦ e' ]]" := (free_evar_subst x e' e) (at level 2, e' at level 200, left associativity,
+  format "e ^[[ 'evar:' x ↦ e' ]]" ) : ml_scope.
+  Notation "e ^[[ 'svar:' X ↦ e' ]]" := (free_svar_subst X e' e) (at level 2, e' at level 200, left associativity,
+  format "e ^[[ 'svar:' X ↦ e' ]]" ) : ml_scope.
+  Notation "e ^ [ e' ]" := (instantiate e e') (at level 2, e' at level 200, left associativity) : ml_scope.
+
+End Notations.
+
+Section subst.
+  Import Substitution.Notations.
+  Context {Σ : Signature}.
 
   (* replace element variable x with de Bruijn index level *)
   Fixpoint evar_quantify (x : evar) (level : db_index)
@@ -164,74 +185,16 @@ Section subst.
              (p : Pattern) : Pattern :=
     patt_mu (svar_quantify X 0 p).
 
+  Open Scope ml_scope.
 
-  
   (* replace de Bruijn index k with element variable n *)
   Definition evar_open (k : db_index) (x : evar) (p : Pattern) : Pattern :=
-    bevar_subst p (patt_free_evar x) k.
+    p^[evar: k ↦ patt_free_evar x].
 
 
   (* replace de Bruijn index k with set variable n *)
   Definition svar_open (k : db_index) (X : svar) (p : Pattern) : Pattern :=
-    bsvar_subst p (patt_free_svar X) k.
-
-  Lemma evar_open_free_evar k n x: evar_open k n (patt_free_evar x) = patt_free_evar x.
-  Proof. reflexivity. Qed.
-  Lemma evar_open_free_svar k n X: evar_open k n (patt_free_svar X) = patt_free_svar X.
-  Proof. reflexivity. Qed.
-  Lemma evar_open_bound_evar k n x: evar_open k n (patt_bound_evar x) = 
-                           match compare_nat x k with
-                           | Nat_less _ _ _ => patt_bound_evar x
-                           | Nat_equal _ _ _ => patt_free_evar n
-                           | Nat_greater _ _ _ => patt_bound_evar (Nat.pred x)
-                           end.
-  Proof.
-    cbn. case_match; done.
-  Qed.
-  Lemma evar_open_bound_svar k n X: evar_open k n (patt_bound_svar X) = patt_bound_svar X.
-  Proof. reflexivity. Qed.
-  Lemma evar_open_sym k n s: evar_open k n (patt_sym s) = patt_sym s.
-  Proof. reflexivity. Qed.
-  Lemma evar_open_app k n ls rs: evar_open k n (patt_app ls rs) = patt_app (evar_open k n ls) (evar_open k n rs).
-  Proof. reflexivity. Qed.
-  Lemma evar_open_bott k n: evar_open k n patt_bott = patt_bott.
-  Proof. reflexivity. Qed.
-  Lemma evar_open_imp k n ls rs: evar_open k n (patt_imp ls rs) = patt_imp (evar_open k n ls) (evar_open k n rs).
-  Proof. reflexivity. Qed.
-  Lemma evar_open_exists k n p': evar_open k n (patt_exists p') = patt_exists (evar_open (S k) n p').
-  Proof. reflexivity. Qed.
-  Lemma evar_open_mu k n p': evar_open k n (patt_mu p') = patt_mu (evar_open k n p').
-  Proof. reflexivity. Qed.
-
-  (* More trivial but useful lemmas *)
-  Lemma svar_open_free_evar k n x: svar_open k n (patt_free_evar x) = patt_free_evar x.
-  Proof. reflexivity. Qed.
-  Lemma svar_open_free_svar k n X: svar_open k n (patt_free_svar X) = patt_free_svar X.
-  Proof. reflexivity. Qed.
-  Lemma svar_open_bound_evar k n x: svar_open k n (patt_bound_evar x) = patt_bound_evar x.
-  Proof. reflexivity. Qed.
-  Lemma svar_open_bound_svar k n X: svar_open k n (patt_bound_svar X) = 
-                                    match compare_nat X k with
-                                    | Nat_less _ _ _ => patt_bound_svar X
-                                    | Nat_equal _ _ _ => patt_free_svar n
-                                    | Nat_greater _ _ _ => patt_bound_svar (Nat.pred X)
-                                    end.
-  Proof.
-    reflexivity.
-  Qed.
-  Lemma svar_open_sym k n s: svar_open k n (patt_sym s) = patt_sym s.
-  Proof. reflexivity. Qed.
-  Lemma svar_open_app k n ls rs: svar_open k n (patt_app ls rs) = patt_app (svar_open k n ls) (svar_open k n rs).
-  Proof. reflexivity. Qed.
-  Lemma svar_open_bott k n: svar_open k n patt_bott = patt_bott.
-  Proof. reflexivity. Qed.
-  Lemma svar_open_imp k n ls rs: svar_open k n (patt_imp ls rs) = patt_imp (svar_open k n ls) (svar_open k n rs).
-  Proof. reflexivity. Qed.
-  Lemma svar_open_exists k n p': svar_open k n (patt_exists p') = patt_exists (svar_open k n p').
-  Proof. reflexivity. Qed.
-  Lemma svar_open_mu k n p': svar_open k n (patt_mu p') = patt_mu (svar_open (S k) n p').
-  Proof. reflexivity. Qed.
-
+    p^[svar: k ↦ patt_free_svar X].
 
   Lemma evar_open_size :
     forall (k : db_index) (n : evar) (p : Pattern),
@@ -384,177 +347,11 @@ Proof using .
 Qed.
 
 
-  (* The following lemmas are trivial but useful for [rewrite !simpl_evar_open]. *)
-
-(******************************************************************************)
-(*****************BOUND ELEMENT VARIABLE SUBSTITUTION**************************)
-  Lemma bevar_subst_free_evar ψ (pf : well_formed_closed ψ) n x :
-    bevar_subst (patt_free_evar x) ψ n = patt_free_evar x.
-  Proof. reflexivity. Qed.
-
-  Lemma bevar_subst_free_svar ψ (pf : well_formed_closed ψ) n X :
-    bevar_subst (patt_free_svar X) ψ n = patt_free_svar X.
-  Proof. reflexivity. Qed.
-
-  Lemma bevar_subst_bound_evar ψ (pf : well_formed_closed ψ) n x :
-    bevar_subst (patt_bound_evar x) ψ n = match compare_nat x n with
-                                          | Nat_less _ _ _ => patt_bound_evar x
-                                          | Nat_equal _ _ _ => ψ
-                                          | Nat_greater _ _ _ => patt_bound_evar (pred x)
-                                          end.
-  Proof.
-    cbn. case_match; done.
-  Qed.
-
-  Lemma bevar_subst_bound_svar ψ (pf : well_formed_closed ψ) n X :
-    bevar_subst (patt_bound_svar X) ψ n = patt_bound_svar X.
-  Proof. reflexivity. Qed.
-
-  Lemma bevar_subst_sym ψ (pf : well_formed_closed ψ) n s :
-    bevar_subst (patt_sym s) ψ n = patt_sym s.
-  Proof. reflexivity. Qed.
-
-  Lemma bevar_subst_app ψ (pf : well_formed_closed ψ) n ls rs :
-    bevar_subst (patt_app ls rs) ψ n = patt_app (bevar_subst ls ψ n) (bevar_subst rs ψ n).
-  Proof. reflexivity. Qed.
-
-  Lemma bevar_subst_bott ψ (pf : well_formed_closed ψ) n:
-    bevar_subst patt_bott ψ n = patt_bott.
-  Proof. reflexivity. Qed.
-
-  Lemma bevar_subst_imp ψ (pf : well_formed_closed ψ) n ls rs :
-    bevar_subst (patt_imp ls rs) ψ n = patt_imp (bevar_subst ls ψ n) (bevar_subst rs ψ n).
-  Proof. reflexivity. Qed.
-
-  Lemma bevar_subst_exists ψ (pf : well_formed_closed ψ) n ϕ :
-    bevar_subst (patt_exists ϕ) ψ n = patt_exists (bevar_subst ϕ ψ (S n)).
-  Proof. reflexivity. Qed.
-
-  Lemma bevar_subst_mu ψ (pf : well_formed_closed ψ) n ϕ :
-    bevar_subst (patt_mu ϕ) ψ n = patt_mu (bevar_subst ϕ ψ n).
-  Proof. reflexivity. Qed.
-
-(******************************************************************************)
-(********************BOUND SET VARIABLE SUBSTITUTION***************************)
-
-  (* More trivial but useful lemmas *)
-  Lemma bsvar_subst_free_evar ψ (pf : well_formed_closed ψ) n x :
-    bsvar_subst (patt_free_evar x) ψ n = patt_free_evar x.
-  Proof. reflexivity. Qed.
-
-  Lemma bsvar_subst_free_svar ψ (pf : well_formed_closed ψ) n X :
-    bsvar_subst (patt_free_svar X) ψ n = patt_free_svar X.
-  Proof. reflexivity. Qed.
-
-  Lemma bsvar_subst_bound_evar ψ (pf : well_formed_closed ψ) n x :
-    bsvar_subst (patt_bound_evar x) ψ n = patt_bound_evar x.
-  Proof. reflexivity. Qed.
-
-  Lemma bsvar_subst_bound_svar ψ (pf : well_formed_closed ψ) n X :
-    bsvar_subst (patt_bound_svar X) ψ n = match compare_nat X n with
-                                          | Nat_less _ _ _ => patt_bound_svar X
-                                          | Nat_equal _ _ _ => ψ
-                                          | Nat_greater _ _ _ => patt_bound_svar (pred X)
-                                          end.
-  Proof.
-    reflexivity.
-  Qed.
-
-  Lemma bsvar_subst_sym ψ (pf : well_formed_closed ψ) n s :
-    bsvar_subst (patt_sym s) ψ n = patt_sym s.
-  Proof. reflexivity. Qed.
-
-  Lemma bsvar_subst_app ψ (pf : well_formed_closed ψ) n ls rs :
-    bsvar_subst (patt_app ls rs) ψ n = patt_app (bsvar_subst ls ψ n) (bsvar_subst rs ψ n).
-  Proof. reflexivity. Qed.
-
-  Lemma bsvar_subst_bott ψ (pf : well_formed_closed ψ) n :
-    bsvar_subst patt_bott ψ n = patt_bott.
-  Proof. reflexivity. Qed.
-
-  Lemma bsvar_subst_imp ψ (pf : well_formed_closed ψ) n ls rs:
-    bsvar_subst (patt_imp ls rs) ψ n = patt_imp (bsvar_subst ls ψ n) (bsvar_subst rs ψ n).
-  Proof. reflexivity. Qed.
-
-  Lemma bsvar_subst_exists ψ (pf : well_formed_closed ψ) n ϕ :
-    bsvar_subst (patt_exists ϕ) ψ n = patt_exists (bsvar_subst ϕ ψ n).
-  Proof. reflexivity. Qed.
-
-  Lemma bsvar_subst_mu ψ (pf : well_formed_closed ψ) n ϕ :
-    bsvar_subst (patt_mu ϕ) ψ n = patt_mu (bsvar_subst ϕ ψ (S n)).
-  Proof. reflexivity. Qed.
-
-(******************************************************************************)
-(*****************FREE ELEMENT VARIABLE SUBSTITUTION***************************)
-
-  Lemma free_evar_subst_exists ψ x ϕ :
-    free_evar_subst (patt_exists ϕ) ψ x = patt_exists (free_evar_subst ϕ ψ x).
-  Proof. reflexivity. Qed.
-
-  Lemma free_evar_subst_mu ψ x ϕ :
-    free_evar_subst (patt_mu ϕ) ψ x = patt_mu (free_evar_subst ϕ ψ x).
-  Proof. reflexivity. Qed.
-
-(******************************************************************************)
-(********************FREE SET VARIABLE SUBSTITUTION****************************)
-
-  Lemma free_svar_subst_exists ψ X ϕ :
-    free_svar_subst (patt_exists ϕ) ψ X = patt_exists (free_svar_subst ϕ ψ X).
-  Proof. reflexivity. Qed.
-
-  Lemma free_svar_subst_mu ψ X ϕ :
-    free_svar_subst (patt_mu ϕ) ψ X = patt_mu (free_svar_subst ϕ ψ X).
-  Proof. reflexivity. Qed.
-
-(******************************************************************************)
-(********************ELEMENT VARIABLE QUANTIFICATION***************************)
-  Lemma evar_quantify_exists n x ϕ :
-    evar_quantify x n (patt_exists ϕ) = patt_exists (evar_quantify x (S n) ϕ).
-  Proof. reflexivity. Qed.
-
-  Lemma evar_quantify_mu n x ϕ :
-    evar_quantify x n (patt_mu ϕ) = patt_mu (evar_quantify x n ϕ).
-  Proof. reflexivity. Qed.
-
-(******************************************************************************)
-(**********************SET VARIABLE QUANTIFICATION*****************************)
-  Lemma svar_quantify_exists N X ϕ :
-    svar_quantify X N (patt_exists ϕ) = patt_exists (svar_quantify X N ϕ).
-  Proof. reflexivity. Qed.
-
-  Lemma svar_quantify_mu N X ϕ :
-    svar_quantify X N (patt_mu ϕ) = patt_mu (svar_quantify X (S N) ϕ).
-  Proof. reflexivity. Qed.
-
-End subst.
-
-Module Notations.
-
-Declare Scope ml_scope.
-Notation "e ^[ 'evar:' dbi ↦ e' ]" := (bevar_subst e e' dbi) (at level 2, e' at level 200, left associativity,
-format "e ^[ 'evar:' dbi ↦ e' ]" ) : ml_scope.
-Notation "e ^[ 'svar:' dbi ↦ e' ]" := (bsvar_subst e e' dbi) (at level 2, e' at level 200, left associativity,
-format "e ^[ 'svar:' dbi ↦ e' ]" ) : ml_scope.
-Notation "e ^[[ 'evar:' x ↦ e' ]]" := (free_evar_subst e e' x) (at level 2, e' at level 200, left associativity,
-format "e ^[[ 'evar:' x ↦ e' ]]" ) : ml_scope.
-Notation "e ^[[ 'svar:' X ↦ e' ]]" := (free_svar_subst e e' X) (at level 2, e' at level 200, left associativity,
-format "e ^[[ 'svar:' X ↦ e' ]]" ) : ml_scope.
-Notation "e ^ [ e' ]" := (instantiate e e') (at level 2, e' at level 200, left associativity) : ml_scope.
-
-End Notations.
-
-Import Notations.
-Open Scope ml_scope.
-
-Section subst.
-    Context {Σ : Signature}.
-
-
 Lemma wfc_ex_aux_bevar_subst :
 forall phi psi n,
   well_formed_closed_ex_aux phi (S n) = true
   -> well_formed_closed_ex_aux psi n = true
-  -> well_formed_closed_ex_aux (bevar_subst phi psi n) n = true.
+  -> well_formed_closed_ex_aux (phi^[evar: n ↦ psi]) n = true.
 Proof.
 intros phi psi n H H0. 
 generalize dependent n. generalize dependent psi.
@@ -578,7 +375,7 @@ Lemma wfc_mu_aux_bevar_subst :
 forall phi psi n n',
   well_formed_closed_mu_aux phi n' = true
   -> well_formed_closed_mu_aux psi n' = true
-  -> well_formed_closed_mu_aux (bevar_subst phi psi n) n' = true.
+  -> well_formed_closed_mu_aux (phi^[evar: n ↦ psi]) n' = true.
 Proof.
 intros phi psi n n' H H0. 
 generalize dependent n. generalize dependent n'. generalize dependent psi.
@@ -601,7 +398,7 @@ Lemma wfc_ex_aux_bsvar_subst :
 forall phi psi n n',
   well_formed_closed_ex_aux phi n = true
   -> well_formed_closed_ex_aux psi n = true
-  -> well_formed_closed_ex_aux (bsvar_subst phi psi n') n = true.
+  -> well_formed_closed_ex_aux (phi^[svar: n' ↦ psi]) n = true.
 Proof.
 intros phi psi n n' H H0. 
 generalize dependent n. generalize dependent n'. generalize dependent psi.
@@ -620,7 +417,7 @@ Lemma wfc_mu_aux_bsvar_subst :
 forall phi psi n',
   well_formed_closed_mu_aux phi (S n') = true
   -> well_formed_closed_mu_aux psi n' = true
-  -> well_formed_closed_mu_aux (bsvar_subst phi psi n') n' = true.
+  -> well_formed_closed_mu_aux (phi^[svar: n' ↦ psi]) n' = true.
 Proof.
 intros phi psi n' H H0. 
 generalize dependent n'. generalize dependent psi.
@@ -774,11 +571,11 @@ Qed.
 Lemma no_neg_occ_db_bevar_subst phi psi dbi1 dbi2:
 well_formed_closed_mu_aux psi 0 = true ->
 no_negative_occurrence_db_b dbi1 phi = true ->
-no_negative_occurrence_db_b dbi1 (bevar_subst phi psi dbi2) = true
+no_negative_occurrence_db_b dbi1 (phi^[evar: dbi2 ↦ psi]) = true
 with no_pos_occ_db_bevar_subst  phi psi dbi1 dbi2:
    well_formed_closed_mu_aux psi 0 = true ->
    no_positive_occurrence_db_b dbi1 phi = true ->
-   no_positive_occurrence_db_b dbi1 (bevar_subst phi psi dbi2) = true.
+   no_positive_occurrence_db_b dbi1 (phi^[evar: dbi2 ↦ psi]) = true.
 Proof.
 - move: dbi1 dbi2.
 induction phi; intros dbi1 dbi2 Hwfcpsi Hnonegphi; cbn in *; auto.
@@ -786,7 +583,7 @@ induction phi; intros dbi1 dbi2 Hwfcpsi Hnonegphi; cbn in *; auto.
 + destruct_and!.
 rewrite -> IHphi1, -> IHphi2; auto.
 + destruct_and!.
-fold (no_positive_occurrence_db_b dbi1 (bevar_subst phi1 psi dbi2)).
+fold (no_positive_occurrence_db_b dbi1 (phi1^[evar: dbi2 ↦ psi]) ).
 rewrite no_pos_occ_db_bevar_subst; auto.
 rewrite -> IHphi2; auto.
 - move: dbi1 dbi2.
@@ -796,7 +593,7 @@ apply wfc_impl_no_pos_occ. assumption.
 + destruct_and!.
 rewrite -> IHphi1, -> IHphi2; auto.
 + destruct_and!.
-fold (no_negative_occurrence_db_b dbi1 (bevar_subst phi1 psi dbi2)).
+fold (no_negative_occurrence_db_b dbi1 (phi1^[evar: dbi2 ↦ psi]) ).
 rewrite no_neg_occ_db_bevar_subst; auto.
 rewrite -> IHphi2; auto.
 Qed.
@@ -806,7 +603,7 @@ forall φ ψ n,
 well_formed_closed_mu_aux ψ 0 = true ->
 well_formed_positive φ = true ->
 well_formed_positive ψ = true ->
-well_formed_positive (bevar_subst φ ψ n) = true.
+well_formed_positive (φ^[evar: n ↦ ψ])  = true.
 Proof.
 induction φ; intros ψ n' H0 H1 H2; cbn in *; auto.
 * break_match_goal; auto.
@@ -959,7 +756,7 @@ Qed.
 
 Lemma well_formed_bevar_subst φ : forall ψ n m,
 m >= n -> well_formed_closed_ex_aux φ n ->
-bevar_subst φ ψ m = φ.
+(φ^[evar: m ↦ ψ]) = φ.
 Proof.
 induction φ; intros ψ n' m' H H0; simpl; auto.
 * simpl in H0. repeat case_match; auto; try lia; congruence.
@@ -975,7 +772,7 @@ Qed.
 
 Lemma well_formed_bsvar_subst φ : forall ψ k m,
 m >= k -> well_formed_closed_mu_aux φ k ->
-bsvar_subst φ ψ m = φ.
+(φ^[svar: m ↦ ψ]) = φ.
 Proof.
 induction φ; intros ψ k' m' H H0; simpl; auto.
 * simpl in H0. repeat case_match; auto; try lia; congruence.
@@ -992,7 +789,7 @@ Qed.
 (* bevar_subst is identity if n does not occur in phi *)
 Corollary bevar_subst_not_occur n ψ ϕ :
 well_formed_closed_ex_aux ϕ n ->
-bevar_subst ϕ ψ n = ϕ.
+(ϕ^[evar: n ↦ ψ]) = ϕ.
 Proof.
 intro H. eapply well_formed_bevar_subst; eauto.
 Qed.
@@ -1008,7 +805,7 @@ Qed.
 (* bsvar_subst is identity if n does not occur in phi *)
 Corollary bsvar_subst_not_occur n ψ ϕ :
 well_formed_closed_mu_aux ϕ n ->
-bsvar_subst ϕ ψ n = ϕ.
+(ϕ^[svar: n ↦ ψ]) = ϕ.
 Proof.
 intro H. eapply well_formed_bsvar_subst; eauto.
 Qed.
@@ -1045,8 +842,8 @@ Qed.
 Lemma bevar_subst_comm_higher :
 forall phi psi1 psi2 n m, 
 n > m -> well_formed_closed_ex_aux psi1 0 -> well_formed_closed_ex_aux psi2 0 ->
-bevar_subst (bevar_subst phi psi1 n) psi2 m = 
-bevar_subst (bevar_subst phi psi2 m) psi1 (pred n).
+(phi^[evar: n ↦ psi1])^[evar: m ↦ psi2] = 
+(phi^[evar: m ↦ psi2])^[evar: pred n ↦ psi1].
 Proof.
 induction phi; intros psi1 psi2 n0 m0 NEQ Hwf1 Hwf2; simpl; auto.
 - repeat case_match; simpl; try rewrite -> Heqc; try rewrite -> Heqc0; auto; subst; try congruence.
@@ -1063,8 +860,8 @@ Qed.
 Lemma bevar_subst_comm_lower :
 forall phi psi1 psi2 n m, 
 n < m -> well_formed_closed_ex_aux psi1 0 -> well_formed_closed_ex_aux psi2 0 ->
-bevar_subst (bevar_subst phi psi1 n) psi2 m = 
-bevar_subst (bevar_subst phi psi2 (S m)) psi1 n.
+(phi^[evar: n ↦ psi1])^[evar: m ↦ psi2] = 
+(phi^[evar: S m ↦ psi2])^[evar: n ↦ psi1].
 Proof.
 induction phi; intros psi1 psi2 n0 m0 NEQ Hwf1 Hwf2; simpl; auto.
 - repeat case_match; simpl; try rewrite -> Heqc; try rewrite -> Heqc0; auto; subst; try congruence.
@@ -1080,8 +877,8 @@ Qed.
 Lemma bsvar_subst_comm_higher :
 forall phi psi1 psi2 n m, 
 n > m -> well_formed_closed_mu_aux psi1 0 -> well_formed_closed_mu_aux psi2 0 ->
-bsvar_subst (bsvar_subst phi psi1 n) psi2 m = 
-bsvar_subst (bsvar_subst phi psi2 m) psi1 (pred n).
+(phi^[svar: n ↦ psi1])^[svar: m ↦ psi2] = 
+(phi^[svar: m ↦ psi2])^[svar: pred n ↦ psi1].
 Proof.
 induction phi; intros psi1 psi2 n0 m0 NEQ Hwf1 Hwf2; simpl; auto.
 - repeat case_match; simpl; try rewrite -> Heqc; try rewrite -> Heqc0; auto; subst; try congruence.
@@ -1098,8 +895,8 @@ Qed.
 Lemma bsvar_subst_comm_lower :
 forall phi psi1 psi2 n m, 
 n < m -> well_formed_closed_mu_aux psi1 0 -> well_formed_closed_mu_aux psi2 0 ->
-bsvar_subst (bsvar_subst phi psi1 n) psi2 m = 
-bsvar_subst (bsvar_subst phi psi2 (S m)) psi1 n.
+(phi^[svar: n ↦ psi1])^[svar: m ↦ psi2] = 
+(phi^[svar: S m ↦ psi2])^[svar: n ↦ psi1].
 Proof.
 induction phi; intros psi1 psi2 n0 m0 NEQ Hwf1 Hwf2; simpl; auto.
 - repeat case_match; simpl; try rewrite -> Heqc; try rewrite -> Heqc0; auto; subst; try congruence.
@@ -1154,8 +951,8 @@ Qed.
 
 Lemma bevar_subst_bsvar_subst phi psi1 psi2 dbi1 dbi2
 : well_formed_closed psi1 -> well_formed_closed psi2 ->
-bevar_subst (bsvar_subst phi psi1 dbi1) psi2 dbi2
-= bsvar_subst (bevar_subst phi psi2 dbi2) psi1 dbi1.
+(phi^[svar: dbi1 ↦ psi1])^[evar: dbi2 ↦ psi2] = 
+(phi^[evar: dbi2 ↦ psi2])^[svar: dbi1 ↦ psi1].
 Proof.
 generalize dependent dbi1. generalize dependent dbi2.
 induction phi; intros dbi1 dbi2 Hwf1 Hwf2; simpl; auto.
@@ -1385,16 +1182,16 @@ Qed.
 
 Corollary evar_open_bsvar_subst m phi1 phi2 dbi X
 : well_formed_closed phi2 ->
-  evar_open m X (bsvar_subst phi1 phi2 dbi)
-  = bsvar_subst (evar_open m X phi1) phi2 dbi.
+  evar_open m X (phi1^[svar: dbi ↦ phi2])
+  = (evar_open m X phi1)^[svar: dbi ↦ phi2].
 Proof.
 intro H. apply bevar_subst_bsvar_subst; auto.
 Qed.
 
 Corollary svar_open_bevar_subst m phi1 phi2 dbi X
 : well_formed_closed phi2 ->
-  svar_open m X (bevar_subst phi1 phi2 dbi)
-  = bevar_subst (svar_open m X phi1) phi2 dbi.
+  svar_open m X (phi1^[evar: dbi ↦ phi2])
+  = (svar_open m X phi1)^[evar: dbi ↦ phi2].
 Proof.
 intro H. apply eq_sym, bevar_subst_bsvar_subst; auto.
 Qed.
@@ -1402,8 +1199,8 @@ Qed.
 Corollary svar_open_bsvar_subst_higher m phi1 phi2 dbi X
 : well_formed_closed phi2 ->
   m < dbi ->
-  svar_open m X (bsvar_subst phi1 phi2 dbi)
-  = bsvar_subst (svar_open m X phi1) phi2 (pred dbi).
+  svar_open m X (phi1^[svar: dbi ↦ phi2])
+  = (svar_open m X phi1)^[svar: pred dbi ↦ phi2].
 Proof.
 intros H H0. apply bsvar_subst_comm_higher; auto.
 unfold well_formed_closed in *. destruct_and!. auto.
@@ -1412,8 +1209,8 @@ Qed.
 Corollary svar_open_bsvar_subst_lower m phi1 phi2 dbi X
 : well_formed_closed phi2 ->
   m > dbi ->
-  svar_open m X (bsvar_subst phi1 phi2 dbi)
-  = bsvar_subst (svar_open (S m) X phi1) phi2 dbi.
+  svar_open m X (phi1^[svar: dbi ↦ phi2])
+  = (svar_open (S m) X phi1)^[svar: dbi ↦ phi2].
 Proof.
 intros H H0. apply bsvar_subst_comm_lower; auto.
 unfold well_formed_closed in *. destruct_and!. auto.
@@ -1422,8 +1219,8 @@ Qed.
 Corollary evar_open_bevar_subst_higher m phi1 phi2 dbi X
 : well_formed_closed_ex_aux phi2 0 ->
   m < dbi ->
-  evar_open m X (bevar_subst phi1 phi2 dbi)
-  = bevar_subst (evar_open m X phi1) phi2 (pred dbi).
+  evar_open m X (phi1^[evar: dbi ↦ phi2])
+  = (evar_open m X phi1)^[evar: pred dbi ↦ phi2].
 Proof.
 intros H H0. apply bevar_subst_comm_higher; auto.
 Qed.
@@ -1431,8 +1228,8 @@ Qed.
 Corollary evar_open_bevar_subst_lower m phi1 phi2 dbi X
 : well_formed_closed phi2 ->
   m > dbi ->
-  evar_open m X (bevar_subst phi1 phi2 dbi)
-  = bevar_subst (evar_open (S m) X phi1) phi2 dbi.
+  evar_open m X (phi1^[evar: dbi ↦ phi2])
+  = (evar_open (S m) X phi1)^[evar: dbi ↦ phi2].
 Proof.
 intros H H0. apply bevar_subst_comm_lower; auto.
 unfold well_formed_closed in *. destruct_and!. auto.
@@ -1442,7 +1239,7 @@ Qed.
 
 Lemma free_svars_bsvar_subst' :
 forall φ ψ dbi X,
-  (X ∈ free_svars (bsvar_subst φ ψ dbi)) <->
+  (X ∈ free_svars (φ^[svar: dbi ↦ ψ])) <->
   ((X ∈ (free_svars ψ) /\ bsvar_occur φ dbi) \/ (X ∈ (free_svars φ))).
 Proof.
 induction φ; intros ψ dbi X; simpl.
@@ -1536,7 +1333,7 @@ Qed.
 
 Lemma free_evars_bevar_subst' :
 forall φ ψ dbi X,
-  (X ∈ free_evars (bevar_subst φ ψ dbi)) <->
+  (X ∈ free_evars (φ^[evar: dbi ↦ ψ])) <->
   ((X ∈ (free_evars ψ) /\ bevar_occur φ dbi) \/ (X ∈ (free_evars φ))).
 Proof.
 induction φ; intros ψ dbi X; simpl.
@@ -1631,7 +1428,7 @@ Qed.
 
 Lemma free_svars_bsvar_subst :
 forall φ ψ dbi,
-free_svars (bsvar_subst φ ψ dbi) ⊆ union (free_svars ψ) (free_svars φ).
+free_svars (φ^[svar: dbi ↦ ψ]) ⊆ union (free_svars ψ) (free_svars φ).
 Proof.
 induction φ; intros ψ dbi; simpl; try set_solver.
 case_match; simpl; set_solver.
@@ -1639,7 +1436,7 @@ Qed.
 
 Lemma free_evars_bevar_subst :
 forall φ ψ dbi,
-free_evars (bevar_subst φ ψ dbi) ⊆ union (free_evars ψ) (free_evars φ).
+free_evars (φ^[evar: dbi ↦ ψ]) ⊆ union (free_evars ψ) (free_evars φ).
 Proof.
 induction φ; intros ψ dbi Hwf; simpl; try set_solver.
 case_match; simpl; set_solver.
@@ -1705,7 +1502,7 @@ Qed.
 
 Lemma free_evar_subst_no_occurrence x p q:
 count_evar_occurrences x p = 0 ->
-free_evar_subst p q x = p.
+p^[[evar:x ↦ q]] = p.
 Proof.
 intros H.
 remember (size' p) as sz.
@@ -1784,7 +1581,7 @@ Lemma well_formed_positive_bevar_subst φ : forall n ψ,
 mu_free φ ->
 well_formed_positive φ = true -> well_formed_positive ψ = true
 ->
-well_formed_positive (bevar_subst φ ψ n) = true.
+well_formed_positive (φ^[evar: n ↦ ψ]) = true.
 Proof.
 induction φ; intros n' ψ H H0 H1; simpl; auto.
 2-3: apply andb_true_iff in H as [E1 E2];
@@ -1794,7 +1591,7 @@ induction φ; intros n' ψ H H0 H1; simpl; auto.
 Qed.
 
 Lemma mu_free_bevar_subst :
-forall φ ψ, mu_free φ -> mu_free ψ -> forall n, mu_free (bevar_subst φ ψ n).
+forall φ ψ, mu_free φ -> mu_free ψ -> forall n, mu_free (φ^[evar: n ↦ ψ]).
 Proof.
 induction φ; intros ψ H H0 n'; simpl; try now constructor.
 * break_match_goal; auto.
@@ -1812,7 +1609,7 @@ Qed.
 
 Theorem evar_open_free_evar_subst_swap :
 forall φ x n ψ y, x <> y -> well_formed ψ ->
-  evar_open n x (free_evar_subst φ ψ y) = free_evar_subst (evar_open n x φ) ψ y.
+  evar_open n x (φ^[[evar: y ↦ ψ]]) = (evar_open n x φ)^[[evar: y ↦ ψ]].
 Proof.
 induction φ; intros x' n' ψ y H H0; simpl; auto.
 * destruct (decide (y = x)); simpl.
@@ -1821,14 +1618,14 @@ induction φ; intros x' n' ψ y H H0; simpl; auto.
   ** reflexivity.
 * cbn. break_match_goal; simpl; auto. destruct (decide (y = x')); auto.
   congruence.
-* unfold evar_open in *. now rewrite -> bevar_subst_app, -> IHφ1, -> IHφ2.
-* unfold evar_open in *. now rewrite -> bevar_subst_imp, -> IHφ1, -> IHφ2.
-* unfold evar_open in *. now rewrite -> bevar_subst_exists, -> IHφ.
-* unfold evar_open in *. now rewrite -> bevar_subst_mu, -> IHφ.
+* unfold evar_open in *. simpl. now rewrite -> IHφ1, -> IHφ2.
+* unfold evar_open in *. simpl. now rewrite -> IHφ1, -> IHφ2.
+* unfold evar_open in *. simpl. now rewrite -> IHφ.
+* unfold evar_open in *. simpl. now rewrite -> IHφ.
 Qed.
 
 Lemma free_evars_free_evar_subst : forall φ ψ x,
-free_evars (free_evar_subst φ ψ x) ⊆ free_evars φ ∪ free_evars ψ.
+free_evars (φ^[[evar: x ↦ ψ]]) ⊆ free_evars φ ∪ free_evars ψ.
 Proof.
 induction φ; intros ψ x'; simpl.
 2-5, 7: apply empty_subseteq.
@@ -1849,7 +1646,7 @@ forall φ x m n ψ,
   m > n ->
   well_formed_closed_ex_aux ψ 0 ->
   well_formed_closed_ex_aux φ m -> x ∉ free_evars φ ->
-  bevar_subst φ ψ n = free_evar_subst (evar_open n x φ) ψ x.
+  φ^[evar: n ↦ ψ] = (evar_open n x φ)^[[evar: x ↦ ψ]].
 Proof.
 induction φ; intros x' m n' ψ H WFψ H0 H1; cbn; auto.
 - destruct (decide (x' = x)); simpl.
@@ -1873,7 +1670,7 @@ forall φ X m n ψ,
   m > n ->
   well_formed_closed_mu_aux ψ 0 ->
   well_formed_closed_mu_aux φ m -> X ∉ free_svars φ ->
-  bsvar_subst φ ψ n = free_svar_subst (svar_open n X φ) ψ X.
+  φ^[svar: n ↦ ψ] = (svar_open n X φ)^[[svar: X ↦ ψ]].
 Proof.
 induction φ; intros x' m n' ψ H WFψ H0 H1; cbn; auto.
 - destruct (decide (x' = x)); simpl.
@@ -1942,7 +1739,7 @@ forall φ ψ n m,
 well_formed_closed_mu_aux φ m = true ->
 well_formed_closed_mu_aux ψ m = true
 ->
-well_formed_closed_mu_aux (bevar_subst φ ψ n) m = true.
+well_formed_closed_mu_aux (φ^[evar: n ↦ ψ]) m = true.
 Proof.
 induction φ; intros ψ n' m H H0; cbn; auto.
 * break_match_goal; simpl in H0, H; simpl; auto.
@@ -1957,7 +1754,7 @@ forall φ ψ n,
 well_formed_closed_ex_aux φ (S n) = true ->
 well_formed_closed_ex_aux ψ n = true
 ->
-well_formed_closed_ex_aux (bevar_subst φ ψ n) n = true.
+well_formed_closed_ex_aux (φ^[evar: n ↦ ψ]) n = true.
 Proof.
 induction φ; intros ψ n' H H0; cbn; auto.
 * break_match_goal; simpl in H0, H; simpl; auto.
@@ -1972,7 +1769,7 @@ Lemma bevar_subst_positive :
 forall φ ψ n, mu_free φ ->
 well_formed_positive φ = true -> well_formed_positive ψ = true
 ->
-well_formed_positive (bevar_subst φ ψ n) = true.
+well_formed_positive (φ^[evar: n ↦ ψ]) = true.
 Proof.
 induction φ; intros ψ n' H H0 H1; cbn; auto.
 * break_match_goal; auto.
@@ -2162,9 +1959,9 @@ Qed.
 Lemma no_neg_occ_db_bsvar_subst phi psi dbi1 dbi2:
 well_formed_closed_mu_aux psi 0 = true -> dbi1 < dbi2 ->
 (no_negative_occurrence_db_b dbi1 phi = true ->
- no_negative_occurrence_db_b dbi1 (bsvar_subst phi psi dbi2) = true)
+ no_negative_occurrence_db_b dbi1 (phi^[svar: dbi2 ↦ psi]) = true)
 /\ (no_positive_occurrence_db_b dbi1 phi = true ->
-    no_positive_occurrence_db_b dbi1 (bsvar_subst phi psi dbi2) = true).
+    no_positive_occurrence_db_b dbi1 (phi^[svar: dbi2 ↦ psi]) = true).
 Proof.
 intros Hwfcpsi.
 move: dbi1 dbi2.
@@ -2227,11 +2024,11 @@ well_formed_closed_mu_aux psi 0 ->
 well_formed_positive phi ->
 (
   no_negative_occurrence_db_b n phi ->
-  well_formed_positive (bsvar_subst phi psi n) )
+  well_formed_positive (phi^[svar: n ↦ psi]) )
 /\ (no_positive_occurrence_db_b n phi ->
     forall phi',
       well_formed_positive phi' ->
-      well_formed_positive (patt_imp (bsvar_subst phi psi n) phi')
+      well_formed_positive (patt_imp (phi^[svar: n ↦ psi]) phi')
    )
 .
 Proof.
@@ -2306,7 +2103,7 @@ induction phi; intros n' Hwfpphi; cbn in *; auto.
 - apply andb_prop in Hwfpphi. destruct Hwfpphi as [Hwfpphi1 Hwfpphi2].
   pose proof (IHphi' := IHphi (S n') Hwfpphi2).
   destruct IHphi' as [IHphi1' IHphi2'].
-  assert (H: no_negative_occurrence_db_b 0 (bsvar_subst phi psi (S n'))).
+  assert (H: no_negative_occurrence_db_b 0 (phi^[svar: S n' ↦ psi])).
   { clear IHphi1' IHphi2'.
     apply no_neg_occ_db_bsvar_subst; auto. lia.
   }
@@ -2328,7 +2125,7 @@ Corollary wfp_bsvar_subst (phi psi : Pattern) :
 well_formed_positive (patt_mu phi) ->
 well_formed_positive psi ->
 well_formed_closed_mu_aux psi 0 ->
-well_formed_positive (bsvar_subst phi psi 0).
+well_formed_positive (phi^[svar: 0 ↦ psi]).
 Proof.
 intros H1 H2 H3.
 simpl in H1.
@@ -2341,12 +2138,9 @@ apply H41.
 apply Hnonegphi.
 Qed.
 
-
-End subst.
-
-Lemma bevar_subst_evar_quantify_free_evar {Σ : Signature} x dbi ϕ:
+Lemma bevar_subst_evar_quantify_free_evar x dbi ϕ:
   well_formed_closed_ex_aux ϕ dbi ->
-  bevar_subst (evar_quantify x dbi ϕ) (patt_free_evar x) dbi  = ϕ.
+  (evar_quantify x dbi ϕ)^[evar: dbi ↦ patt_free_evar x] = ϕ.
 Proof.
   move: dbi.
   induction ϕ; intros dbi Hwf; simpl in *; auto.
@@ -2367,9 +2161,9 @@ Proof.
   - rewrite IHϕ;[assumption|reflexivity].
 Qed.
 
-Lemma bsvar_subst_svar_quantify_free_svar {Σ : Signature} X dbi ϕ:
+Lemma bsvar_subst_svar_quantify_free_svar X dbi ϕ:
   well_formed_closed_mu_aux ϕ dbi ->
-  bsvar_subst (svar_quantify X dbi ϕ) (patt_free_svar X) dbi  = ϕ.
+  (svar_quantify X dbi ϕ)^[svar: dbi ↦ (patt_free_svar X)]  = ϕ.
 Proof.
   move: dbi.
   induction ϕ; intros dbi Hwf; simpl in *; auto.
@@ -2392,9 +2186,9 @@ Qed.
 
 
 
-Lemma free_svar_subst_fresh {Σ : Signature} phi psi X:
+Lemma free_svar_subst_fresh phi psi X:
   svar_is_fresh_in X phi ->
-  free_svar_subst phi psi X = phi.
+  phi^[[svar: X ↦ psi]] = phi.
 Proof.
   intros Hfresh.
   unfold svar_is_fresh_in in Hfresh.
@@ -2419,10 +2213,10 @@ Proof.
 Qed.
 
 
-Lemma wfc_mu_free_svar_subst {Σ : Signature} level ϕ ψ X:
+Lemma wfc_mu_free_svar_subst level ϕ ψ X:
   well_formed_closed_mu_aux ϕ level ->
   well_formed_closed_mu_aux ψ level ->
-  well_formed_closed_mu_aux (free_svar_subst ϕ ψ X) level = true.
+  well_formed_closed_mu_aux (ϕ^[[svar: X ↦ ψ]]) level = true.
 Proof.
   intros Hϕ Hψ.
   move: level Hϕ Hψ.
@@ -2438,13 +2232,10 @@ Proof.
   - rewrite IHϕ; auto. eapply well_formed_closed_mu_aux_ind. 2: exact Hψ. lia.
 Qed.
 
-#[export]
- Hint Resolve wfc_mu_free_svar_subst : core.
-
-Lemma wfc_ex_free_svar_subst {Σ : Signature} level ϕ ψ X:
+Lemma wfc_ex_free_svar_subst level ϕ ψ X:
   well_formed_closed_ex_aux ϕ level ->
   well_formed_closed_ex_aux ψ level ->
-  well_formed_closed_ex_aux (free_svar_subst ϕ ψ X) level = true.
+  well_formed_closed_ex_aux (ϕ^[[svar: X ↦ ψ]]) level = true.
 Proof.
   intros Hϕ Hψ.
   move: level Hϕ Hψ.
@@ -2460,13 +2251,10 @@ Proof.
   - rewrite IHϕ; auto. eapply well_formed_closed_ex_aux_ind. 2: exact Hψ. lia.
 Qed.
 
-#[export]
- Hint Resolve wfc_mu_free_svar_subst : core.
-
-Lemma wfc_ex_free_evar_subst_2 {Σ : Signature} level ϕ ψ X:
+Lemma wfc_ex_free_evar_subst_2 level ϕ ψ x:
   well_formed_closed_ex_aux ϕ level ->
   well_formed_closed_ex_aux ψ level ->
-  well_formed_closed_ex_aux (free_evar_subst ϕ ψ X) level = true.
+  well_formed_closed_ex_aux (ϕ^[[evar: x ↦ ψ]]) level = true.
 Proof.
   intros Hϕ Hψ.
   move: level Hϕ Hψ.
@@ -2482,14 +2270,10 @@ Proof.
   - rewrite IHϕ; auto. eapply well_formed_closed_ex_aux_ind. 2: exact Hψ. lia.
 Qed.
 
-#[export]
- Hint Resolve wfc_ex_free_evar_subst_2 : core.
-
-
-Lemma wfc_mu_free_evar_subst {Σ : Signature} level ϕ ψ x:
+Lemma wfc_mu_free_evar_subst level ϕ ψ x:
 well_formed_closed_mu_aux ϕ level ->
 well_formed_closed_mu_aux ψ level ->
-well_formed_closed_mu_aux (free_evar_subst ϕ ψ x) level = true.
+well_formed_closed_mu_aux (ϕ^[[evar: x ↦ ψ]]) level = true.
 Proof.
 intros Hϕ Hψ.
 move: level Hϕ Hψ.
@@ -2508,7 +2292,7 @@ induction ϕ; intros level Hϕ Hψ; simpl in *; auto.
 Qed.
 
 
-Lemma wf_evar_open_from_wf_ex {Σ : Signature} x ϕ:
+Lemma wf_evar_open_from_wf_ex x ϕ:
   well_formed (patt_exists ϕ) ->
   well_formed (evar_open 0 x ϕ).
 Proof.
@@ -2521,7 +2305,7 @@ Proof.
 Qed.
 
 
-Lemma evar_open_size' {Σ : Signature} :
+Lemma evar_open_size' :
   forall (k : db_index) (n : evar) (p : Pattern),
     size' (evar_open k n p) = size' p.
 Proof.
@@ -2534,7 +2318,7 @@ Proof.
   rewrite (IHp k); reflexivity.
 Qed.
 
-Lemma svar_open_size' {Σ : Signature} :
+Lemma svar_open_size' :
   forall (k : db_index) (n : svar) (p : Pattern),
     size' (svar_open k n p) = size' p.
 Proof.
@@ -2549,12 +2333,11 @@ Qed.
 
 Check fold_left.
 Definition bcmcloseex
-    {Σ : Signature}
     (l : list (prod db_index evar))
     (ϕ : Pattern) : Pattern
 := fold_left (λ ϕ' p, evar_open p.1 p.2 ϕ') l ϕ.
 
-Lemma bcmcloseex_append {Σ : Signature} (l₁ l₂ : list (prod db_index evar)) (ϕ : Pattern) :
+Lemma bcmcloseex_append (l₁ l₂ : list (prod db_index evar)) (ϕ : Pattern) :
   bcmcloseex (l₁ ++ l₂) ϕ = bcmcloseex l₂ (bcmcloseex l₁ ϕ).
 Proof.
   unfold bcmcloseex. rewrite fold_left_app. reflexivity.
@@ -2575,7 +2358,6 @@ Proof.
 Qed.
 *)
 Lemma bcmcloseex_bott
-  {Σ : Signature}
   (l : list (prod db_index evar))
   : bcmcloseex l patt_bott = patt_bott.
 Proof.
@@ -2585,7 +2367,6 @@ Proof.
 Qed.
 
 Lemma bcmcloseex_sym
-  {Σ : Signature}
   (l : list (prod db_index evar))
   (s : symbols)
   : bcmcloseex l (patt_sym s) = (patt_sym s).
@@ -2596,7 +2377,6 @@ Proof.
 Qed.
 
 Lemma bcmcloseex_imp
-  {Σ : Signature}
   (l : list (prod db_index evar))
   (p q : Pattern)
   : bcmcloseex l (patt_imp p q) = patt_imp (bcmcloseex l p) (bcmcloseex l q).
@@ -2608,7 +2388,6 @@ Proof.
 Qed.
 
 Lemma bcmcloseex_app
-  {Σ : Signature}
   (l : list (prod db_index evar))
   (p q : Pattern)
   : bcmcloseex l (patt_app p q) = patt_app (bcmcloseex l p) (bcmcloseex l q).
@@ -2620,7 +2399,6 @@ Proof.
 Qed.
 
 Lemma bcmcloseex_ex
-  {Σ : Signature}
   (l : list (prod db_index evar))
   (q : Pattern)
   : bcmcloseex l (patt_exists q) = patt_exists (bcmcloseex (map (λ p, (S p.1,p.2)) l) q).
@@ -2632,7 +2410,6 @@ Proof.
 Qed.
 
 Lemma bcmcloseex_mu
-  {Σ : Signature}
   (l : list (prod db_index evar))
   (q : Pattern)
   : bcmcloseex l (patt_mu q) = patt_mu (bcmcloseex l q).
@@ -2643,7 +2420,7 @@ Proof.
   { simpl. rewrite IHl. reflexivity. }
 Qed.
 
-Lemma wfc_ex_aux_S_bevar_subst_fe {Σ : Signature} k ϕ x:
+Lemma wfc_ex_aux_S_bevar_subst_fe k ϕ x:
   well_formed_closed_ex_aux ϕ^[evar:k↦patt_free_evar x] k = true ->
   well_formed_closed_ex_aux ϕ (S k) = true.  
 Proof.
@@ -2654,7 +2431,7 @@ Proof.
   { destruct_and!. rewrite IHϕ1;[assumption|]. rewrite IHϕ2;[assumption|]. reflexivity. }
 Qed.
 
-Lemma wfc_ex_aux_evar_open_gt {Σ : Signature} dbi x k ϕ:
+Lemma wfc_ex_aux_evar_open_gt dbi x k ϕ:
   k > dbi ->
   well_formed_closed_ex_aux (evar_open dbi x ϕ) k ->
   well_formed_closed_ex_aux ϕ (S k).
@@ -2688,7 +2465,7 @@ Proof.
   }
 Qed.
 
-Lemma wfc_ex_aux_evar_open_lt {Σ : Signature} dbi x k ϕ:
+Lemma wfc_ex_aux_evar_open_lt dbi x k ϕ:
   k < dbi ->
   well_formed_closed_ex_aux (evar_open dbi x ϕ) k = true ->
   well_formed_closed_ex_aux ϕ (S dbi) = true.
@@ -2721,7 +2498,7 @@ Proof.
   }
 Qed.
 
-Lemma evar_open_twice_not_occur {Σ : Signature} n x y ϕ:
+Lemma evar_open_twice_not_occur n x y ϕ:
   bevar_occur ϕ n = false ->
   evar_open n y (evar_open n x ϕ) = evar_open n x (evar_open (S n) y ϕ).
 Proof.
@@ -2755,7 +2532,7 @@ Proof.
   }
 Qed.
 
-Lemma wfc_ex_aux_bcmcloseex {Σ : Signature} l k ϕ:
+Lemma wfc_ex_aux_bcmcloseex l k ϕ:
   Forall (λ p : nat * evar, p.1 ≤ k) l ->
   well_formed_closed_ex_aux (bcmcloseex l (patt_exists ϕ)) k = true ->
   well_formed_closed_ex_aux (bcmcloseex (map (λ p : nat * evar, (S p.1, p.2)) l) ϕ) (S k) = true.
@@ -2773,8 +2550,8 @@ Proof.
   }
 Qed.
 
-Lemma free_svars_free_evar_subst {Σ : Signature} ϕ x ψ:
-  free_svars (free_evar_subst ϕ ψ x) ⊆ free_svars ϕ ∪ free_svars ψ.
+Lemma free_svars_free_evar_subst ϕ x ψ:
+  free_svars (ϕ^[[evar: x ↦ ψ]]) ⊆ free_svars ϕ ∪ free_svars ψ.
 Proof.
   induction ϕ; simpl; try set_solver.
   {
@@ -2788,3 +2565,12 @@ Proof.
   }
 Qed.
 
+End subst.
+
+
+#[export]
+ Hint Resolve wfc_mu_free_svar_subst : core.
+#[export]
+ Hint Resolve wfc_mu_free_svar_subst : core.
+#[export]
+ Hint Resolve wfc_ex_free_evar_subst_2 : core.
